src/Congress.v
@@ -11,13 +11,14 @@ From SmartContracts Require Import Oak.
 From SmartContracts Require Import Monads.
 From RecordUpdate Require Import RecordUpdate.
 (* This is included last to default things to list rather than map/set *)
-From Coq Require Import List. 
+From Coq Require Import List.
 
 Import MapNotations.
 Import ListNotations.
 Import RecordSetNotations.
 
 Open Scope Z.
+Set Primitive Projections.
 
 Definition ProposalId := nat.
 
@@ -53,15 +54,15 @@ Record Setup :=
   }.
 
 Inductive Msg :=
-| TransferOwnership : Address -> Msg
-| ChangeRules : Rules -> Msg
-| AddMember : Address -> Msg
-| RemoveMember : Address -> Msg
-| CreateProposal : list CongressAction -> Msg
-| VoteForProposal : ProposalId -> Msg
-| VoteAgainstProposal : ProposalId -> Msg
-| RetractVote : ProposalId -> Msg
-| FinishProposal : ProposalId -> Msg.
+  | transfer_ownership : Address -> Msg
+  | change_rules : Rules -> Msg
+  | add_member : Address -> Msg
+  | remove_member : Address -> Msg
+  | create_proposal : list CongressAction -> Msg
+  | vote_for_proposal : ProposalId -> Msg
+  | vote_against_proposal : ProposalId -> Msg
+  | retract_vote : ProposalId -> Msg
+  | finish_proposal : ProposalId -> Msg.
 
 Record State :=
   build_state {
@@ -79,7 +80,7 @@ Instance eta_state : Settable _ :=
                                <*> proposals
                                <*> next_proposal_id
                                <*> members)%settable.
-  
+
 Definition version : Version := 1%nat.
 
 Definition validate_rules (rules : Rules) : bool :=
@@ -92,7 +93,7 @@ Definition validate_rules (rules : Rules) : bool :=
 Definition init (ctx : ContractCallContext) (setup : Setup) : option State :=
   if validate_rules setup.(setup_rules) then
     Some {| owner := ctx.(ctx_from);
-            state_rules := setup.(setup_rules); 
+            state_rules := setup.(setup_rules);
             proposals := []%map;
             next_proposal_id := 1%nat;
             members := {}%set |}
@@ -125,7 +126,7 @@ Definition vote_on_proposal
   let new_proposal := proposal[[votes := new_votes]][[vote_result := new_vote_result]] in
   Some (state[[proposals ::= MapInterface.add pid new_proposal]]).
 
-Definition retract_vote
+Definition do_retract_vote
            (voter : Address)
            (pid : ProposalId)
            (state : State)
@@ -143,7 +144,7 @@ Definition congress_action_to_chain_action (act : CongressAction) : ChainAction 
   | cact_call to amt msg => act_call to amt msg
   end.
 
-Definition finish_proposal
+Definition do_finish_proposal
            (pid : ProposalId)
            (state : State)
            (chain : Chain)
@@ -181,37 +182,147 @@ Definition receive
   let is_from_member := (sender \in state.(members))%set in
   let without_actions := option_map (fun new_state => (new_state, [ ])) in
   match is_from_owner, is_from_member, maybe_msg with
-  | true, _, Some (TransferOwnership new_owner) =>
+  | true, _, Some (transfer_ownership new_owner) =>
         Some (state[[owner := new_owner]], [ ])
 
-  | true, _, Some (ChangeRules new_rules) =>
+  | true, _, Some (change_rules new_rules) =>
         if validate_rules new_rules then
             Some (state[[state_rules := new_rules]], [ ])
         else
             None
 
-  | true, _, Some (AddMember new_member) =>
+  | true, _, Some (add_member new_member) =>
         Some (state[[members ::= SetInterface.add new_member]], [ ])
 
-  | true, _, Some (RemoveMember old_member) =>
+  | true, _, Some (remove_member old_member) =>
         Some (state[[members ::= SetInterface.remove old_member]], [ ])
 
-  | _, true, Some (CreateProposal actions) =>
+  | _, true, Some (create_proposal actions) =>
         Some (add_proposal actions chain state, [ ])
 
-  | _, true, Some (VoteForProposal pid) =>
+  | _, true, Some (vote_for_proposal pid) =>
         without_actions (vote_on_proposal sender pid 1 state)
 
-  | _, true, Some (VoteAgainstProposal pid) =>
+  | _, true, Some (vote_against_proposal pid) =>
         without_actions (vote_on_proposal sender pid (-1) state)
 
-  | _, true, Some (RetractVote pid) =>
-        without_actions (retract_vote sender pid state)
+  | _, true, Some (retract_vote pid) =>
+        without_actions (do_retract_vote sender pid state)
 
-  | _, _, Some (FinishProposal pid) =>
-        finish_proposal pid state chain
- 
+  | _, _, Some (finish_proposal pid) =>
+        do_finish_proposal pid state chain
+
   | _, _, _ =>
         None
-    
+
   end.
+
+Definition deserialize_rules (v : OakValue) : option Rules :=
+  do '((a, b), c) <- deserialize v;
+  Some (build_rules a b c).
+
+Program Instance rules_equivalence : OakTypeEquivalence Rules :=
+  {| serialize r := let (a, b, c) := r in serialize (a, b, c);
+     (* Why does
+     deserialize v :=
+       do '((a, b), c) <- deserialize v;
+       Some (build_rules a b c); |}.
+       not work here? *)
+     deserialize := deserialize_rules; |}.
+
+Program Instance setup_equivalence : OakTypeEquivalence Setup :=
+  {| serialize s := serialize s.(setup_rules);
+     deserialize or :=
+       do rules <- deserialize or;
+       Some (build_setup rules); |}.
+
+Definition deserialize_congress_action (v : OakValue) : option CongressAction :=
+  do val <- deserialize v;
+  Some (match val with
+  | inl (to, amount) => cact_transfer to amount
+  | inr (to, amount, msg) => cact_call to amount msg
+  end).
+
+Program Instance congress_action_equivalence : OakTypeEquivalence CongressAction :=
+  {| serialize ca :=
+       serialize
+         match ca with
+         | cact_transfer to amount => inl (to, amount)
+         | cact_call to amount msg => inr (to, amount, msg)
+         end;
+     deserialize := deserialize_congress_action; |}.
+Next Obligation.
+  unfold deserialize_congress_action.
+  rewrite ote_equivalence.
+  destruct x; reflexivity.
+Qed.
+
+Definition deserialize_proposal (v : OakValue) : option Proposal :=
+  do '(a, b, c, d) <- deserialize v;
+  Some (build_proposal a b c d).
+
+Program Instance proposal_equivalence : OakTypeEquivalence Proposal :=
+  {| serialize p :=
+       let (a, b, c, d) := p in
+       serialize (a, b, c, d);
+     deserialize := deserialize_proposal;
+  |}.
+Next Obligation.
+  unfold deserialize_proposal.
+  rewrite ote_equivalence.
+  destruct x; reflexivity.
+Qed.
+
+Definition serialize_msg (m : Msg) : OakValue :=
+  serialize
+    match m with
+    | transfer_ownership a => (0, serialize a)
+    | change_rules r => (1, serialize r)
+    | add_member a => (2, serialize a)
+    | remove_member a => (3, serialize a)
+    | create_proposal l => (4, serialize l)
+    | vote_for_proposal pid => (5, serialize pid)
+    | vote_against_proposal pid => (6, serialize pid)
+    | retract_vote pid => (7, serialize pid)
+    | finish_proposal pid => (8, serialize pid)
+    end.
+
+Definition deserialize_msg (v : OakValue) : option Msg :=
+  do '(tag, v) <- deserialize v;
+  match tag with
+  | 0 => option_map transfer_ownership (deserialize v)
+  | 1 => option_map change_rules (deserialize v)
+  | 2 => option_map add_member (deserialize v)
+  | 3 => option_map remove_member (deserialize v)
+  | 4 => option_map create_proposal (deserialize v)
+  | 5 => option_map vote_for_proposal (deserialize v)
+  | 6 => option_map vote_against_proposal (deserialize v)
+  | 7 => option_map retract_vote (deserialize v)
+  | 8 => option_map finish_proposal (deserialize v)
+  | _ => None
+  end.
+
+Program Instance msg_equivalence : OakTypeEquivalence Msg :=
+  {| serialize := serialize_msg; deserialize := deserialize_msg; |}.
+Next Obligation.
+  unfold serialize_msg, deserialize_msg.
+  destruct x; repeat (simpl; rewrite ote_equivalence); reflexivity.
+Qed.
+
+Definition serialize_state (s : State) : OakValue :=
+  let (a, b, c, d, e) := s in
+  serialize (a, b, c, d, e).
+
+Definition deserialize_state (v : OakValue) : option State :=
+  do '(a, b, c, d, e) <- deserialize v;
+  Some (build_state a b c d e).
+
+Program Instance state_equivalence : OakTypeEquivalence State :=
+  {| serialize := serialize_state; deserialize := deserialize_state; |}.
+Next Obligation.
+  unfold serialize_state, deserialize_state.
+  destruct x; repeat (simpl; rewrite ote_equivalence); reflexivity.
+Qed.
+
+Definition contract : Contract Setup Msg State :=
+  build_contract version init receive.
