src/LocalBlockchain.v
@@ -2,107 +2,278 @@ From Coq Require Import ZArith.
 From SmartContracts Require Import Blockchain.
 From SmartContracts Require Import Oak.
 From SmartContracts Require Import Monads.
+From RecordUpdate Require Import RecordUpdate.
 From Containers Require Import Maps.
 From Coq Require Import List.
+From SmartContracts Require Import Extras.
 
+Import RecordSetNotations.
 Import ListNotations.
 (* Note that [ ] or nil is needed for the empty list
    in this file as [] parses an empty map *)
 
-Local Record ContractInstance :=
-  {
-    inst_state_ty : OakType;
-    inst_msg_ty : OakType;
-    inst_state : interp_type inst_state_ty;
-    inst_receive : ContractCallContext -> interp_type inst_state_ty ->
-                   option (interp_type inst_msg_ty) -> ChainAction;
-  }.
-
 Local Record ChainUpdate :=
-  {
-    upd_block : Block;
+  build_chain_update {
     (* Contracts that had their states updated and the new state *)
-    upd_contracts : Map[Address, ContractInstance];
-    (* Contracts deployed in this block *)
-    upd_deployments : Map[Address, ContractDeployment];
+    upd_contracts : Map[Address, OakValue];
     (* All transactions caused by update, including internal txs
        (due to contract execution) *)
     upd_txs : list Tx;
   }.
 
-Inductive LocalChain :=
-  {
+Instance eta_chain_update : Settable _ :=
+  mkSettable
+    ((constructor build_chain_update) <*> upd_contracts
+                                      <*> upd_txs)%settable.
+
+(* Contains information about the chain that contracts should have access
+   to. This does not contain definitions of contracts, for instance. *)
+Record LocalChain :=
+  build_local_chain {
+    (* List of blocks and updates. Generally such lists have the
+       same length, except during contract execution, where lc_updates
+       is one ahead of lc_blocks (to facilitate tracking state within
+       the block) *)
+    lc_blocks : list Block;
     lc_updates : list ChainUpdate;
   }.
+
+Instance eta_local_chain : Settable _ :=
+  mkSettable
+    ((constructor build_local_chain) <*> lc_blocks
+                                     <*> lc_updates)%settable.
+
+(* Contains full information about a chain, including contracts *)
+Record LocalChainEnvironment :=
+  build_local_chain_environment {
+    lce_lc : LocalChain;
+    lce_contracts : list (Address * WeakContract);
+  }.
+
+Instance eta_local_chain_environment : Settable _ :=
+  mkSettable
+    ((constructor build_local_chain_environment) <*> lce_lc
+                                                 <*> lce_contracts)%settable.
 
 Definition genesis_block : Block :=
   {| block_header := {| block_number := 0; |};
      block_txs := nil |}.
 
 Definition initial_chain : LocalChain :=
-  {| lc_updates :=
-       [{| upd_block := genesis_block;
-           upd_contracts := []%map;
-           upd_deployments := []%map;
+  {| lc_blocks := [genesis_block];
+     lc_updates :=
+       [{| upd_contracts := []%map;
            upd_txs := nil |}]
   |}.
 
 Definition lc_chain_at (lc : LocalChain) (bid : BlockId) : option LocalChain :=
-  let is_old u := u.(upd_block).(block_header).(block_number) <=? bid in
-  let new_updates := filter is_old lc.(lc_updates) in
-  match new_updates with
-  | hd :: tl => if hd.(upd_block).(block_header).(block_number) =? bid
-                then Some {| lc_updates := new_updates |}
+  let is_old '(b, u) := b.(block_header).(block_number) <=? bid in
+  let zipped := rev (combine (rev lc.(lc_blocks)) (rev lc.(lc_updates))) in
+  let zipped_at := filter is_old zipped in
+  let '(at_blocks, at_updates) := split zipped_at in
+  match at_blocks with
+  | hd :: _ => if hd.(block_header).(block_number) =? bid
+                then Some {| lc_blocks := at_blocks; lc_updates := at_updates; |}
                 else None
   | nil => None
   end.
 
 Definition lc_block_at (lc : LocalChain) (bid : BlockId) : option Block :=
-  let blocks := map upd_block lc.(lc_updates) in
+  let blocks := lc.(lc_blocks) in
   find (fun b => b.(block_header).(block_number) =? bid) blocks.
 
 Definition lc_head_block (lc : LocalChain) : Block :=
-  match lc.(lc_updates) with
-  | hd :: _ => hd.(upd_block)
+  match lc.(lc_blocks) with
+  | hd :: _ => hd
   | nil => genesis_block
   end.
 
 Definition lc_incoming_txs (lc : LocalChain) (addr : Address) : list Tx :=
-  let all_txs := flat_map (fun u => u.(upd_block).(block_txs)) lc.(lc_updates) in
+  let all_txs := flat_map (fun u => u.(upd_txs)) lc.(lc_updates) in
   let is_inc tx := (tx.(tx_to) =? addr)%address in
   filter is_inc all_txs.
 
 Definition lc_outgoing_txs (lc : LocalChain) (addr : Address) : list Tx :=
-  let all_txs := flat_map (fun u => u.(upd_block).(block_txs)) lc.(lc_updates) in
+  let all_txs := flat_map (fun u => u.(upd_txs)) lc.(lc_updates) in
   let is_out tx := (tx.(tx_from) =? addr)%address in
   filter is_out all_txs.
 
-Local Definition find_first {A : Type} (f : ChainUpdate -> option A) (lc : LocalChain)
-  : option A :=
-  let opts := map f lc.(lc_updates) in
-  let is_some o := match o with | Some _ => true | None => false end in
-  match filter is_some opts with
-  | hd :: _ => hd
-  | _ => None
-  end.
-
-Definition lc_contract_deployment (lc : LocalChain) (addr : Address)
-  : option ContractDeployment :=
-  find_first (fun u => u.(upd_deployments)[addr]%map) lc.
-
 Definition lc_contract_state (lc : LocalChain) (addr : Address)
   : option OakValue :=
-  let get_state_oak_value u :=
-      do c <- u.(upd_contracts)[addr]%map;
-      Some (build_oak_value c.(inst_state_ty) c.(inst_state)) in
-  find_first get_state_oak_value lc.
+  find_first (fun u => u.(upd_contracts)[addr]%map) lc.(lc_updates).
 
-Definition local_chain_impl : ChainInterface :=
+Definition lc_interface : ChainInterface :=
   {| ci_chain_type := LocalChain;
      ci_chain_at := lc_chain_at;
      ci_head_block := lc_head_block;
      ci_incoming_txs := lc_incoming_txs;
      ci_outgoing_txs := lc_outgoing_txs;
-     ci_contract_deployment := lc_contract_deployment;
      ci_contract_state := lc_contract_state;
   |}.
+
+
+Section ExecuteActions.
+  Context (initial_lce : LocalChainEnvironment).
+
+  Local Record ExecutionContext :=
+    build_execution_context {
+      block_txs : list Tx;
+      new_update : ChainUpdate;
+      new_contracts : list (Address * WeakContract);
+    }.
+
+  Local Instance eta_execution_context : Settable _ :=
+    mkSettable
+      ((constructor build_execution_context) <*> block_txs
+                                             <*> new_update
+                                             <*> new_contracts)%settable.
+
+  Let make_acc_lce ec :=
+    let new_lc := (initial_lce.(lce_lc))[[lc_updates ::= cons ec.(new_update)]] in
+    let new_contracts := ec.(new_contracts) ++ initial_lce.(lce_contracts) in
+    {| lce_lc := new_lc; lce_contracts := new_contracts |}.
+
+  Let make_acc_c lce : Chain :=
+    build_chain lc_interface lce.(lce_lc).
+
+  Let verify_amount (c : Chain) (addr : Address) (amt : Amount)
+    : option unit :=
+    if (amt <=? account_balance c addr)%nat
+    then Some tt
+    else None.
+
+  Let find_contract addr lce :=
+    option_map snd (find (fun p => fst p =? addr) lce.(lce_contracts)).
+
+  Let verify_no_contract addr lce :=
+    match find_contract addr lce with
+    | Some _ => None
+    | None => Some tt
+    end.
+
+  Fixpoint execute_action
+          (act : Address (*from*) * ChainAction)
+          (ec : ExecutionContext)
+          (gas : nat)
+          (record : bool) (* should the action be recorded in the block *)
+          {struct gas}
+    : option ExecutionContext :=
+    match gas, act with
+    | 0, _ => None
+    | S gas, (from, act) =>
+      let acc_lce := make_acc_lce ec in
+      let acc_c := make_acc_c acc_lce in
+      let deploy_contract amount (wc : WeakContract) setup :=
+          do verify_amount acc_c from amount;
+          let contract_addr := 0 in (* todo *)
+          do verify_no_contract contract_addr acc_lce;
+          let ctx := {| ctx_chain := acc_c;
+                        ctx_from := from;
+                        ctx_contract_address := contract_addr;
+                        ctx_amount := amount |} in
+          let (ver, init, recv) := wc in
+          do state <- init ctx setup;
+          let contract_deployment :=
+                {| deployment_version := ver;
+                   deployment_setup := setup |} in
+          let new_tx := {| tx_from := from;
+                           tx_to := contract_addr;
+                           tx_amount := amount;
+                           tx_body := tx_deploy contract_deployment |} in
+          let new_cu :=
+              ec.(new_update)[[upd_contracts ::= MapInterface.add contract_addr state]]
+                             [[upd_txs ::= cons new_tx]] in
+          let new_contract := (contract_addr, wc) in
+          let new_ec :=
+              ec[[new_update := new_cu]]
+                [[new_contracts ::= cons new_contract]] in
+          let new_ec := if record then new_ec[[block_txs ::= cons new_tx]] else new_ec in
+          Some new_ec in
+
+      let send_or_call to amount msg_opt :=
+          do verify_amount acc_c from amount;
+          let new_tx := {| tx_from := from;
+                           tx_to := to;
+                           tx_amount := amount;
+                           tx_body :=
+                             match msg_opt with
+                             | Some msg => tx_call msg
+                             | None => tx_empty
+                             end |} in
+          let new_cu := ec.(new_update)[[upd_txs ::= cons new_tx]] in
+          let new_ec := ec[[new_update := new_cu]] in
+          let new_ec := if record then new_ec[[block_txs ::= cons new_tx]] else new_ec in
+          match find_contract to acc_lce with
+          | None => Some new_ec
+          | Some wc =>
+            let acc_lce := make_acc_lce new_ec in
+            let acc_c := make_acc_c acc_lce in
+            let contract_addr := to in
+            do state <- lc_contract_state acc_lce.(lce_lc) contract_addr;
+            let (ver, init, recv) := wc in
+            let ctx := {| ctx_chain := acc_c;
+                          ctx_from := from;
+                          ctx_contract_address := contract_addr;
+                          ctx_amount := amount |} in
+            do '(new_state, resp_actions) <- recv ctx state msg_opt;
+            let new_cu :=
+                ec.(new_update)[[upd_contracts ::= MapInterface.add to new_state]]
+                               [[upd_txs ::= cons new_tx]] in
+            let new_ec := ec[[new_update := new_cu]] in
+            let new_ec := if record then new_ec[[block_txs ::= cons new_tx]] else new_ec in
+            let fix go acts cur_ec :=
+                match acts with
+                  | nil => Some cur_ec
+                  | hd :: tl =>
+                    do cur_ec <- execute_action (contract_addr, hd) cur_ec gas false;
+                    go tl cur_ec
+                end in
+            go resp_actions new_ec
+          end in
+
+      match act with
+      | act_deploy amount wc setup => deploy_contract amount wc setup
+      | act_transfer to amount => send_or_call to amount None
+      | act_call to amount msg => send_or_call to amount (Some msg)
+      end
+    end.
+
+  Definition execute_actions
+             (coinbase : Tx)
+             (actions : list (Address * ChainAction))
+             (gas : nat)
+    : option LocalChainEnvironment :=
+    let fix go acts ec :=
+        match acts with
+        | nil => Some ec
+        | hd :: tl =>
+          do ec <- execute_action hd ec gas true;
+          go tl ec
+        end in
+    let empty_ec := {| block_txs := [coinbase];
+                       new_update := {| upd_contracts := []%map;
+                                        upd_txs := [coinbase] |};
+                       new_contracts := nil |} in
+    do ec <- go actions empty_ec;
+    let new_lce := make_acc_lce ec in
+    let recorded_txs := ec.(block_txs) in
+    let hdr := {| block_number := length (initial_lce.(lce_lc).(lc_blocks)) |} in
+    let block := build_block hdr recorded_txs in
+    let new_lce := new_lce[[lce_lc := new_lce.(lce_lc)[[lc_blocks ::= cons block]]]] in
+    Some new_lce.
+End ExecuteActions.
+
+(* Adds a block to the chain by executing the specified chain actions.
+   Returns the new chain if the execution succeeded (for instance,
+   transactions need enough funds, contracts should not reject, etc. *)
+Definition add_block
+           (coinbase : Address)
+           (actions : list (Address (*from*) * ChainAction))
+           (lce : LocalChainEnvironment)
+  : option LocalChainEnvironment :=
+  let coinbase_tx :=
+      {| tx_from := 0;
+         tx_to := coinbase;
+         tx_amount := 50;
+         tx_body := tx_empty |} in
+  execute_actions lce coinbase_tx actions 10.
