src/Oak.v
@@ -1,13 +1,17 @@
 From Coq Require Import ZArith.
 From Containers Require Import Sets Maps.
+From Containers Require SetProperties.
+From SmartContracts Require Import Monads.
+From Coq Require Import List.
+From Coq Require Import Setoid.
 
 Inductive OakType :=
   | oak_empty : OakType
   | oak_unit : OakType
   | oak_int : OakType
   | oak_bool : OakType
-  | oak_sum : OakType -> OakType -> OakType
   | oak_pair : OakType -> OakType -> OakType
+  | oak_sum : OakType -> OakType -> OakType
   | oak_list : OakType -> OakType
   | oak_set : OakType -> OakType
   | oak_map : OakType -> OakType -> OakType.
@@ -15,40 +19,54 @@ Inductive OakType :=
 Definition eq_oak_type_dec (t1 t2 : OakType) : {t1 = t2} + {t1 <> t2}.
 Proof. decide equality. Defined.
 
+Proposition eq_oak_type_dec_refl (x : OakType) :
+  eq_oak_type_dec x x = left eq_refl.
+Proof.
+  induction x;
+    try simpl; try rewrite IHx; try rewrite IHx1; try rewrite IHx2; reflexivity.
+Qed.
+
 Program Instance empty_set_strict_order
   : OrderedType.StrictOrder (fun (_ _ : Empty_set) => False) (@eq Empty_set).
 Solve Obligations with contradiction.
 Program Instance empty_set_ordered_type : UsualOrderedType Empty_set.
 Solve Obligations with contradiction.
 
-Local Fixpoint interp_type_with_ordering (t : OakType) : {T : Type & OrderedType T} :=
+Set Primitive Projections.
+Local Record OakInterpretation :=
+  build_interpretation {
+    oi_ty : Type;
+    oi_order : OrderedType oi_ty;
+  }.
+
+Local Fixpoint interp_type_with_ordering (t : OakType) : OakInterpretation :=
   match t with
-  | oak_empty => existT OrderedType Empty_set _
-  | oak_unit => existT OrderedType unit _
-  | oak_int => existT OrderedType Z _
-  | oak_bool => existT OrderedType bool _
+  | oak_empty => build_interpretation Empty_set _
+  | oak_unit => build_interpretation unit _
+  | oak_int => build_interpretation Z _
+  | oak_bool => build_interpretation bool _
   | oak_sum a b =>
-    let 'existT aT _ := interp_type_with_ordering a in
-    let 'existT bT _ := interp_type_with_ordering b in
-    existT OrderedType (aT + bT)%type _
+    let (aT, _) := interp_type_with_ordering a in
+    let (bT, _) := interp_type_with_ordering b in
+    build_interpretation (aT + bT)%type _
   | oak_pair a b =>
-    let 'existT aT _ := interp_type_with_ordering a in
-    let 'existT bT _ := interp_type_with_ordering b in
-    existT OrderedType (aT * bT)%type _
+    let (aT, _) := interp_type_with_ordering a in
+    let (bT, _) := interp_type_with_ordering b in
+    build_interpretation (aT * bT)%type _
   | oak_list a =>
-    let 'existT aT _ := interp_type_with_ordering a in
-    existT OrderedType (list aT) _
+    let (aT, _) := interp_type_with_ordering a in
+    build_interpretation (list aT) _
   | oak_set a =>
-    let 'existT aT _ := interp_type_with_ordering a in
-    existT OrderedType (set aT) _
+    let (aT, _) := interp_type_with_ordering a in
+    build_interpretation (set aT) _
   | oak_map a b =>
-    let 'existT aT _ := interp_type_with_ordering a in
-    let 'existT bT _ := interp_type_with_ordering b in
-    existT OrderedType Map[aT, bT] _
+    let (aT, _) := interp_type_with_ordering a in
+    let (bT, _) := interp_type_with_ordering b in
+    build_interpretation Map[aT, bT] _
   end.
 
 Definition interp_type (t : OakType) : Type :=
-  projT1 (interp_type_with_ordering t).
+  oi_ty (interp_type_with_ordering t).
 
 Record OakValue :=
   build_oak_value {
@@ -63,6 +81,170 @@ Proof.
   - subst. exact (Some val).
   - exact None.
 Defined.
+
+(* Defines that a type can be serialized into OakValue and deserialized from it,
+   and that these are inverses *)
+Class OakTypeEquivalence (ty : Type) :=
+  {
+    serialize : ty -> OakValue;
+    deserialize : OakValue -> option ty;
+    ote_equivalence : forall (x : ty), deserialize (serialize x) = Some x;
+  }.
+
+Global Opaque serialize deserialize ote_equivalence.
+
+Definition make_trivial_equiv (ot : OakType) : OakTypeEquivalence (interp_type ot).
+Proof.
+  refine {| serialize := build_oak_value ot;
+            deserialize := extract_oak_value ot;
+            ote_equivalence := _ |}.
+  intros x.
+  unfold extract_oak_value.
+  rewrite eq_oak_type_dec_refl.
+  reflexivity.
+Defined.
+
+Instance oak_empty_equivalence : OakTypeEquivalence Empty_set :=
+  make_trivial_equiv oak_empty.
+
+Instance oak_unit_equivalence : OakTypeEquivalence unit :=
+  make_trivial_equiv oak_unit.
+
+Instance oak_int_equivalence : OakTypeEquivalence Z :=
+  make_trivial_equiv oak_int.
+
+Instance oak_bool_equivalence : OakTypeEquivalence bool :=
+  make_trivial_equiv oak_bool.
+
+Program Instance oak_nat_equivalence : OakTypeEquivalence nat :=
+  {| serialize n := serialize (Z.of_nat n);
+     deserialize z := do z' <- deserialize z; Some (Z.to_nat z'); |}.
+Next Obligation.
+  rewrite ote_equivalence.
+  simpl.
+  rewrite Nat2Z.id.
+  reflexivity.
+Qed.
+
+Program Instance oak_value_equivalence : OakTypeEquivalence OakValue :=
+  {| serialize v := v;
+     deserialize v := Some v; |}.
+
+Generalizable Variables A B.
+Program Instance oak_sum_equivalence
+        `{e_a : OakTypeEquivalence A}
+        `{e_b : OakTypeEquivalence B}
+  : OakTypeEquivalence (A + B)%type :=
+  {| serialize s :=
+       let (is_left, ov) :=
+           match s with
+           | inl l => (true, serialize l)
+           | inr r => (false, serialize r)
+           end in
+       build_oak_value (oak_pair oak_bool ov.(oak_value_type)) (is_left, ov.(oak_value));
+     deserialize os :=
+       match os with
+       | build_oak_value (oak_pair oak_bool v) (b, val) =>
+         if b
+         then do a <- @deserialize _ e_a (build_oak_value v val);
+              Some (inl a)
+         else do b <- @deserialize _ e_b (build_oak_value v val);
+              Some (inr b)
+       | _ => None
+       end;
+  |}.
+Next Obligation.
+  destruct x as [a | b]; rewrite ote_equivalence; reflexivity.
+  (*
+  - change ({| oak_value_type := oak_value_type (serialize a);
+               oak_value := oak_value (serialize a) |}) with (serialize a).
+
+    rewrite ote_equivalence.
+  *)
+Qed.
+
+Program Instance oak_pair_equivalence
+        `{e_a : OakTypeEquivalence A}
+        `{e_b : OakTypeEquivalence B}
+  : OakTypeEquivalence (A * B)%type :=
+  {| serialize '(a, b) :=
+       let 'build_oak_value a_oty a_val := serialize a in
+       let 'build_oak_value b_oty b_val := serialize b in
+       build_oak_value (oak_pair a_oty b_oty) (a_val, b_val);
+     deserialize op :=
+       match op with
+       | build_oak_value (oak_pair a_ty b_ty) (a_val, b_val) =>
+         do a <- @deserialize _ e_a (build_oak_value a_ty a_val);
+         do b <- @deserialize _ e_b (build_oak_value b_ty b_val);
+         Some (a, b)
+       | _ => None
+       end;
+  |}.
+Next Obligation.
+  repeat rewrite ote_equivalence.
+  reflexivity.
+Qed.
+
+Program Instance oak_list_equivalence
+        `{OakTypeEquivalence A}
+  : OakTypeEquivalence (list A) :=
+  {| serialize l :=
+       let go a acc :=
+           let 'build_oak_value a_oty a_val := serialize a in
+           let 'build_oak_value acc_oty acc_val := acc in
+           build_oak_value (oak_pair a_oty acc_oty) (a_val, acc_val) in
+       fold_right go (build_oak_value oak_unit tt) l;
+     deserialize ol :=
+       let fix aux (ty : OakType) (val : interp_type ty) : option (list A) :=
+           match ty with
+           | oak_pair hd_ty tl_ty =>
+             let pair : interp_type hd_ty * interp_type tl_ty := ltac:(subst; exact val) in
+             let (hd_val, tl_val) := pair in
+             do hd <- deserialize (build_oak_value hd_ty hd_val);
+             do tl <- aux tl_ty tl_val;
+             Some (hd :: tl)
+           | oak_unit => Some nil
+           | _ => None
+           end in
+       let 'build_oak_value ol_ty ol_val := ol in
+       aux ol_ty ol_val;
+  |}.
+Solve Obligations with split; discriminate.
+Next Obligation.
+  induction x as [| hd tl IHl].
+  - reflexivity.
+  - simpl.
+    rewrite IHl.
+    rewrite ote_equivalence.
+    reflexivity.
+Qed.
+
+Program Instance oak_map_equivalence
+        `{OakTypeEquivalence A}
+        `{OrderedType A}
+        `{OakTypeEquivalence B}
+  : OakTypeEquivalence Map[A, B] :=
+  {| serialize m := serialize (MF.to_list m);
+     deserialize om :=
+       do elems <- deserialize om;
+       Some (MF.of_list elems);
+  |}.
+Next Obligation.
+  (* TODO: Need to use setoids here... *)
+  Admitted.
+
+Program Instance oak_set_equivalence
+        `{OakTypeEquivalence A}
+        `{OrderedType A}
+  : OakTypeEquivalence (SetInterface.set A) :=
+  {| serialize s := serialize (SetProperties.to_list s);
+     deserialize os :=
+       do elems <- deserialize os;
+       Some (SetProperties.of_list elems);
+  |}.
+Next Obligation.
+  (* TODO: Setoids ... *)
+  Admitted.
 
 (*
 Examples:
