src/Extras.v
@@ -1,0 +1,12 @@
+From Coq Require Import List.
+Import ListNotations.
+
+Fixpoint find_first {A B : Type} (f : A -> option B) (l : list A)
+  : option B :=
+  match l with
+  | hd :: tl => match f hd with
+                | Some b => Some b
+                | None => find_first f tl
+                end
+  | [] => None
+  end.
